theories/Operational/Awkernel/Minimal/WorkloadCandidateSource.v
@@ -1,0 +1,353 @@
+From Stdlib Require Import List Bool Arith Arith.PeanoNat Lia.
+Import ListNotations.
+From RocqSched Require Import Foundation.Base.
+From RocqSched Require Import Operational.Common.OSCandidateSourceContract.
+From RocqSched Require Import Operational.Common.OSLocalAdapterContract.
+From RocqSched Require Import Operational.Common.OSSchedulerViewContract.
+From RocqSched Require Import Operational.Common.OSProjectionInterface.
+From RocqSched Require Import Operational.Common.ConcreteExecution.
+From RocqSched Require Import Operational.Common.State.
+From RocqSched Require Import Operational.Common.Step.
+From RocqSched Require Import Operational.Awkernel.Minimal.MinimalProjection.
+From RocqSched Require Import Operational.Awkernel.Minimal.CapturedTraceSyntax.
+From RocqSched Require Import Operational.Awkernel.Minimal.WorkloadAcceptance.
+From RocqSched Require Import Operational.Awkernel.Minimal.WorkloadCandidateTable.
+
+Definition empty_sched_trace_entry : AwkernelSchedTraceEntry :=
+  mkAwkernelSchedTraceEntry 0 EvStutter None [] false None.
+
+Definition workload_execution_matches_sched_trace
+    {P : OSLabeledProjection AwkernelState}
+    (ex : labeled_concrete_execution P 2)
+    (sched_trace : list AwkernelSchedTraceEntry) : Prop :=
+  forall t,
+    os_to_op_state (osl_to_os_projection P) (lce_trace ex t) =
+    awk_to_op_state
+      (awk_sched_trace_entry_to_state (nth t sched_trace empty_sched_trace_entry)).
+
+Definition accepted_workload_candidate_source_family
+    (task_trace : list AwkernelTaskTraceEntry)
+    (sched_trace : list AwkernelSchedTraceEntry)
+    (table : list (list JobId)) : Prop :=
+  accepted_workload_sched_trace_family task_trace sched_trace /\
+  workload_candidate_table_contract sched_trace table.
+
+Lemma job_in_listb_sound :
+  forall j xs,
+    job_in_listb j xs = true ->
+    In j xs.
+Proof.
+  intros j xs.
+  induction xs as [|x xs IH]; intros Hin; simpl in Hin.
+  - discriminate.
+  - apply Bool.orb_true_iff in Hin.
+    destruct Hin as [Heq | Hin].
+    + apply Nat.eqb_eq in Heq. subst x. left. reflexivity.
+    + right. apply IH. exact Hin.
+Qed.
+
+Lemma job_in_optionb_sound :
+  forall oj j,
+    job_in_optionb oj j = true ->
+    oj = Some j.
+Proof.
+  intros [j'|] j H; simpl in H.
+  - apply Nat.eqb_eq in H. subst j'. reflexivity.
+  - discriminate.
+Qed.
+
+Lemma all_jobs_includedb_sound :
+  forall jobs cand j,
+    all_jobs_includedb jobs cand = true ->
+    In j jobs ->
+    In j cand.
+Proof.
+  intros jobs.
+  induction jobs as [|j' jobs IH]; intros cand j Hin Hall; simpl in *.
+  - contradiction.
+  - apply Bool.andb_true_iff in Hin as [Hj' Hrest].
+    destruct Hall as [Heq | Hinjobs].
+    + subst j'. apply job_in_listb_sound. exact Hj'.
+    + apply IH; assumption.
+Qed.
+
+Lemma all_candidates_visibleb_sound :
+  forall row cand j,
+    all_candidates_visibleb row cand = true ->
+    In j cand ->
+    row_candidate_visibleb row j = true.
+Proof.
+  intros row cand.
+  induction cand as [|j' cand IH]; intros j Hvisible Hin; simpl in *.
+  - contradiction.
+  - apply Bool.andb_true_iff in Hvisible as [Hhead Htail].
+    destruct Hin as [Heq | Hin].
+    + subst j. exact Hhead.
+    + apply IH; assumption.
+Qed.
+
+Lemma row_candidate_visibleb_sound :
+  forall row j,
+    aste_cpu row < 2 ->
+    row_candidate_visibleb row j = true ->
+    op_job_visible 2 (awk_to_op_state (awk_sched_trace_entry_to_state row)) j.
+Proof.
+  intros row j Hcpu Hvisible.
+  unfold row_candidate_visibleb in Hvisible.
+  apply Bool.orb_true_iff in Hvisible.
+  destruct Hvisible as [Hvisible | Htarget].
+  - apply Bool.orb_true_iff in Hvisible.
+    destruct Hvisible as [Hcurrent | Hrunnable].
+    + left.
+      exists (aste_cpu row).
+      split; [assumption|].
+      unfold awk_sched_trace_entry_to_state, awk_to_op_state.
+      simpl.
+      destruct (aste_current row) as [j'|] eqn:Hcur; simpl in Hcurrent; try discriminate.
+      apply Nat.eqb_eq in Hcurrent.
+      subst j'.
+      rewrite Nat.eqb_refl.
+      reflexivity.
+    + right. left.
+      unfold awk_sched_trace_entry_to_state, awk_to_op_state.
+      simpl.
+      apply job_in_listb_sound.
+      exact Hrunnable.
+  - right. right.
+    exists (aste_cpu row).
+    split; [assumption|].
+    unfold awk_sched_trace_entry_to_state, awk_to_op_state.
+    simpl.
+    destruct (aste_dispatch_target row) as [j'|] eqn:Hdispatch;
+      simpl in Htarget; try discriminate.
+    apply Nat.eqb_eq in Htarget.
+    subst j'.
+    rewrite Nat.eqb_refl.
+    reflexivity.
+Qed.
+
+Lemma awk_sched_trace_state_current_inv :
+  forall row c j,
+    op_current (awk_to_op_state (awk_sched_trace_entry_to_state row)) c = Some j ->
+    aste_current row = Some j /\ c = aste_cpu row.
+Proof.
+  intros row c j Hcur.
+  unfold awk_sched_trace_entry_to_state, awk_to_op_state in Hcur.
+  simpl in Hcur.
+  destruct (aste_current row) as [j'|] eqn:Hentry; simpl in Hcur; try discriminate.
+  destruct (Nat.eqb c (aste_cpu row)) eqn:Hcpu; inversion Hcur; subst j.
+  apply Nat.eqb_eq in Hcpu.
+  split; assumption.
+Qed.
+
+Lemma awk_sched_trace_state_dispatch_target_inv :
+  forall row c j,
+    op_dispatch_target (awk_to_op_state (awk_sched_trace_entry_to_state row)) c = Some j ->
+    aste_dispatch_target row = Some j /\ c = aste_cpu row.
+Proof.
+  intros row c j Htarget.
+  unfold awk_sched_trace_entry_to_state, awk_to_op_state in Htarget.
+  simpl in Htarget.
+  destruct (aste_dispatch_target row) as [j'|] eqn:Hentry;
+    simpl in Htarget; try discriminate.
+  destruct (Nat.eqb c (aste_cpu row)) eqn:Hcpu; inversion Htarget; subst j.
+  apply Nat.eqb_eq in Hcpu.
+  split; assumption.
+Qed.
+
+Lemma Forall2_nth_error_some :
+  forall A B (R : A -> B -> Prop) xs ys n x y,
+    Forall2 R xs ys ->
+    nth_error xs n = Some x ->
+    nth_error ys n = Some y ->
+    R x y.
+Proof.
+  intros A B R xs ys n.
+  revert xs ys.
+  induction n as [|n IH]; intros xs ys x y Hfor Hx Hy.
+  - destruct Hfor; simpl in *; try discriminate.
+    inversion Hx; inversion Hy; subst.
+    assumption.
+  - destruct Hfor; simpl in *; try discriminate.
+    eapply IH; eauto.
+Qed.
+
+Lemma workload_candidate_table_contract_nth :
+  forall sched_trace table t row cand,
+    workload_candidate_table_contract sched_trace table ->
+    nth_error sched_trace t = Some row ->
+    nth_error table t = Some cand ->
+    workload_candidate_row_contract row cand.
+Proof.
+  intros sched_trace table t row cand [_ Hrows] Hrow Hcand.
+  eapply Forall2_nth_error_some; eauto.
+Qed.
+
+Lemma candidate_source_of_table_in_bounds :
+  forall table t j,
+    In j (candidate_source_of_table table (fun _ => mkJob 0 0 0 0 1) 2 (fun _ _ => None) t) ->
+    t < length table.
+Proof.
+  intros table t j Hin.
+  unfold candidate_source_of_table in Hin.
+  destruct (lt_dec t (length table)) as [Hlt | Hnlt].
+  - exact Hlt.
+  - rewrite nth_overflow in Hin by lia.
+    contradiction.
+Qed.
+
+Lemma accepted_workload_candidate_source_sound_from_contract :
+  forall (P : OSLabeledProjection AwkernelState)
+         jobs adm
+         (C : awk_local_adapter_contract P jobs adm 2)
+         sched_trace table,
+    Forall (fun entry => aste_cpu entry < 2) sched_trace ->
+    workload_candidate_table_contract sched_trace table ->
+    workload_execution_matches_sched_trace (olac_execution C) sched_trace ->
+    awk_labeled_concrete_candidate_source_contract
+      P
+      jobs
+      2
+      (candidate_source_of_table table)
+      (olac_execution C).
+Proof.
+  intros P jobs adm C sched_trace table Hcpus Htable Hmatch.
+  refine
+    {| lccsc_candidates_visible := _;
+       lccsc_current_in_candidates := _;
+       lccsc_runnable_in_candidates := _;
+       lccsc_dispatch_target_in_candidates := _;
+       lccsc_prefix_extensional := _ |}.
+  - intros t j Hin.
+    pose proof (candidate_source_of_table_in_bounds table t j Hin) as Ht.
+    assert (Ht_rows : t < length sched_trace).
+    { rewrite (proj1 Htable). exact Ht. }
+    assert (Hrow : nth_error sched_trace t = Some (nth t sched_trace empty_sched_trace_entry)).
+    { apply nth_error_nth'. exact Ht_rows. }
+    assert (Hcand : nth_error table t = Some (nth t table [])).
+    { apply nth_error_nth'. exact Ht. }
+    pose proof (workload_candidate_table_contract_nth
+                  sched_trace table t
+                  (nth t sched_trace empty_sched_trace_entry)
+                  (nth t table [])
+                  Htable Hrow Hcand) as Hrow_contract.
+    destruct Hrow_contract as [_ [Hvisible [_ [_ _]]]].
+    rewrite (Hmatch t).
+    eapply row_candidate_visibleb_sound.
+    + eapply Forall_nth; eauto.
+    + eapply all_candidates_visibleb_sound; eauto.
+  - intros t c j Hlt Hcur.
+    rewrite Hmatch in Hcur.
+    destruct (lt_dec t (length sched_trace)) as [Ht | Ht].
+    + assert (Hrow : nth_error sched_trace t = Some (nth t sched_trace empty_sched_trace_entry)).
+      { apply nth_error_nth'. exact Ht. }
+      assert (Ht_table : t < length table).
+      { rewrite <- (proj1 Htable). exact Ht. }
+      assert (Hcand : nth_error table t = Some (nth t table [])).
+      { apply nth_error_nth'. exact Ht_table. }
+      pose proof (workload_candidate_table_contract_nth
+                    sched_trace table t
+                    (nth t sched_trace empty_sched_trace_entry)
+                    (nth t table [])
+                    Htable Hrow Hcand) as Hrow_contract.
+      destruct Hrow_contract as [_ [_ [Hcurrent [_ _]]]].
+      destruct (awk_sched_trace_state_current_inv
+                  (nth t sched_trace empty_sched_trace_entry) c j Hcur) as [Hentry _].
+      unfold option_candidate_includedb in Hcurrent.
+      rewrite Hentry in Hcurrent.
+      simpl in Hcurrent.
+      apply job_in_listb_sound.
+      exact Hcurrent.
+    + rewrite nth_overflow in Hcur by lia.
+      discriminate.
+  - intros t j Hin.
+    rewrite Hmatch in Hin.
+    destruct (lt_dec t (length sched_trace)) as [Ht | Ht].
+    + assert (Hrow : nth_error sched_trace t = Some (nth t sched_trace empty_sched_trace_entry)).
+      { apply nth_error_nth'. exact Ht. }
+      assert (Ht_table : t < length table).
+      { rewrite <- (proj1 Htable). exact Ht. }
+      assert (Hcand : nth_error table t = Some (nth t table [])).
+      { apply nth_error_nth'. exact Ht_table. }
+      pose proof (workload_candidate_table_contract_nth
+                    sched_trace table t
+                    (nth t sched_trace empty_sched_trace_entry)
+                    (nth t table [])
+                    Htable Hrow Hcand) as Hrow_contract.
+      destruct Hrow_contract as [_ [_ [_ [Hrunnable _]]]].
+      unfold awk_sched_trace_entry_to_state, awk_to_op_state in Hin.
+      simpl in Hin.
+      eapply all_jobs_includedb_sound; eauto.
+    + rewrite nth_overflow in Hin by lia.
+      contradiction.
+  - intros t c j Hlt Hdispatch.
+    rewrite Hmatch in Hdispatch.
+    destruct (lt_dec t (length sched_trace)) as [Ht | Ht].
+    + assert (Hrow : nth_error sched_trace t = Some (nth t sched_trace empty_sched_trace_entry)).
+      { apply nth_error_nth'. exact Ht. }
+      assert (Ht_table : t < length table).
+      { rewrite <- (proj1 Htable). exact Ht. }
+      assert (Hcand : nth_error table t = Some (nth t table [])).
+      { apply nth_error_nth'. exact Ht_table. }
+      pose proof (workload_candidate_table_contract_nth
+                    sched_trace table t
+                    (nth t sched_trace empty_sched_trace_entry)
+                    (nth t table [])
+                    Htable Hrow Hcand) as Hrow_contract.
+      destruct Hrow_contract as [_ [_ [_ [_ Htarget]]]].
+      destruct (awk_sched_trace_state_dispatch_target_inv
+                  (nth t sched_trace empty_sched_trace_entry) c j Hdispatch) as [Hentry _].
+      unfold option_candidate_includedb in Htarget.
+      rewrite Hentry in Htarget.
+      simpl in Htarget.
+      apply job_in_listb_sound.
+      exact Htarget.
+    + rewrite nth_overflow in Hdispatch by lia.
+      discriminate.
+  - intros s1 s2 t Hprefix.
+    apply candidate_source_of_table_prefix_extensional.
+    exact Hprefix.
+Qed.
+
+Lemma accepted_workload_candidate_source_sound :
+  forall (P : OSLabeledProjection AwkernelState)
+         jobs adm
+         (C : awk_local_adapter_contract P jobs adm 2)
+         task_trace sched_trace table,
+    accepted_workload_candidate_source_family task_trace sched_trace table ->
+    workload_execution_matches_sched_trace (olac_execution C) sched_trace ->
+    awk_labeled_concrete_candidate_source_contract
+      P
+      jobs
+      2
+      (candidate_source_of_table table)
+      (olac_execution C).
+Proof.
+  intros P jobs adm C task_trace sched_trace table
+         [Haccepted Htable] Hmatch.
+  eapply accepted_workload_candidate_source_sound_from_contract.
+  - eapply accepted_workload_sched_trace_family_cpus_in_range.
+    exact Haccepted.
+  - exact Htable.
+  - exact Hmatch.
+Qed.
+
+Definition accepted_workload_candidate_source_adapter_contract
+    (P : OSLabeledProjection AwkernelState)
+    jobs adm
+    (C : awk_local_adapter_contract P jobs adm 2)
+    task_trace sched_trace table
+    (Hfamily : accepted_workload_candidate_source_family task_trace sched_trace table)
+    (Hmatch : workload_execution_matches_sched_trace (olac_execution C) sched_trace)
+    : awk_local_candidate_source_adapter_contract
+        P
+        (candidate_source_of_table table)
+        jobs
+        adm
+        2 :=
+  {|
+    olcsac_base := C;
+    olcsac_candidates :=
+      accepted_workload_candidate_source_sound
+        P jobs adm C task_trace sched_trace table Hfamily Hmatch;
+  |}.
